lawyer/nonblocking/examples/queue/dequeuer/dequeue_ghost.v
@@ -170,22 +170,23 @@ Section DequeueGhost.
       destruct LL as [-> ?]. by iFrame.
   Qed.
 
-  Lemma queue_elems_interp_shorten (PE: val -> iProp Σ) hq h:
-    queue_elems_interp PE hq h ⊣⊢ queue_elems_interp PE hq (h + 1) ∗ from_option (PE ∘ fst ∘ snd) True (hq !! h). 
-  Proof using.
-    rewrite /queue_elems_interp.
-    rewrite Nat.add_comm'  -skipn_skipn.
-    rewrite -{3}(Nat.add_0_r h). rewrite -lookup_drop.
-    remember (drop h hq) as l. rewrite -Heql. clear Heql. 
-    destruct l.
-    { simpl. iSplit; set_solver. }
-    simpl. rewrite drop_0. iSplit; iIntros "[$ $]".
-  Qed.
+  (* Lemma queue_elems_interp_shorten (PE: val -> iProp Σ) hq h: *)
+  (*   queue_elems_interp PE hq h ⊣⊢ queue_elems_interp PE hq (h + 1) ∗ from_option (PE ∘ fst ∘ snd) True (hq !! h).  *)
+  (* Proof using. *)
+  (*   rewrite /queue_elems_interp. *)
+  (*   rewrite Nat.add_comm'  -skipn_skipn. *)
+  (*   rewrite -{3}(Nat.add_0_r h). rewrite -lookup_drop. *)
+  (*   remember (drop h hq) as l. rewrite -Heql. clear Heql.  *)
+  (*   destruct l. *)
+  (*   { simpl. iSplit; set_solver. } *)
+  (*   simpl. rewrite drop_0. iSplit; iIntros "[$ $]". *)
+  (* Qed. *)
+
+  Context (PE: val -> iProp Σ) {PERS_PE: forall v, Persistent (PE v)}. 
 
   Lemma dequeue_upd_head_post (τ : locale heap_lang)
     (h : nat) (ph : loc) (vh : val) (nxh : loc) (fl : nat)
     (hq : HistQueue) (t br : nat) (rop : option nat) (hist : read_hist)
-    PE
   (ORDER : hq_state_wf h t br fl)
   (HTH : hq !! h = Some (ph, (vh, nxh)))
   (NEMPTY : t ≠ h)
@@ -205,7 +206,7 @@ Section DequeueGhost.
   (∃ nfl : HistNode, ⌜hq !! fl = Some nfl⌝ ∗ FreeLater q_sq ↦ #nfl.1 ∗
            hn_interp nfl) -∗
   dangle_auth None -∗
-  ohv_interp -∗
+  ohv_interp PE -∗
   read_hist_interp hist rop h br fl None -∗
   ((∃ pt0 : loc, read_head_resources t br pt0 None ∗ rop_token)
          ∨ read_head_token) -∗
@@ -216,7 +217,7 @@ Section DequeueGhost.
            ⊤ ∖ ↑queue_ns,⊤}=∗ emp) -∗
   Head q_sq ↦{1 / 2} #nxh -∗
   Head q_sq ↦{1 / 2} #nxh -∗
-  queue_elems_interp PE hq h -∗
+  queue_elems_interp PE hq -∗
   |={⊤ ∖ ↑queue_ns,⊤}=> 
     (@me_exact _ q_me_h (h + 1) ∗ @me_exact _ q_me_fl fl ∗ Head q_sq ↦{1 / 2} #nxh ∗
      dangle_frag (Some h)) ∗
@@ -226,8 +227,8 @@ Section DequeueGhost.
        ∨ ith_rp i rs_aborted ∨ ith_rp i (rs_proc (Some rsp_completed)))
       (* ∗ PE vh *) (** it is moved from queue_elems_interp to dangle_interp *)
   .
-  Proof using. 
-    iIntros "#HTH CH CFL DFRAG HQ AUTHS Q TAIL DUMMY BR FL DAUTH OHV RHI RH TOK CLOS HEAD HEAD' EI".
+  Proof using PERS_PE. 
+    iIntros "#HTH CH CFL DFRAG HQ AUTHS Q TAIL DUMMY BR FL DAUTH OHV RHI RH TOK CLOS HEAD HEAD' #EI".
 
     iMod (dangle_update _ _ (Some h) with "[$] [$]") as "[DAUTH DFRAG]".
 
@@ -247,9 +248,8 @@ Section DequeueGhost.
     iDestruct (take_snapshot with "[$]") as "#SHT".
     iDestruct "SHT" as "(_&_&#BR_LB&_)".
 
-    iDestruct (queue_elems_interp_shorten with "EI") as "[EI' PEv]".
-    rewrite HTH /=.
-    (* iFrame "PEv".  *)
+    (* iDestruct (queue_elems_interp_shorten with "EI") as "[EI' PEv]". *)
+    (* rewrite HTH /=. *)    
 
     rewrite /read_hist_interp. iDestruct "RHI" as "(ROPA & ROP & RHIST & %RH_WF & #OLDS)". 
     rewrite /rop_interp.
@@ -274,8 +274,9 @@ Section DequeueGhost.
         - iDestruct "FROM_BR" as "([-> ->] & -> & ?)". lia. } 
 
       iClear "HTH".
-      iMod ("CLOS" with "[-]") as "_"; [| done].      
-      iFrame "QI AUTHS OHV HQ RH DAUTH TOK RHIST ROPA EI'". iNext.
+      iMod ("CLOS" with "[-]") as "_"; [| done].
+      iDestruct (queue_elems_interp_get with "EI") as "PEv"; eauto.
+      iFrame "QI AUTHS OHV HQ RH DAUTH TOK RHIST ROPA EI". iNext.
       rewrite Nat.add_sub. rewrite HTH /=. 
       
       iSplit.
@@ -336,13 +337,14 @@ Section DequeueGhost.
       
       iSplit.
       { iPureIntro. red. red in ORDER. repeat split; try lia. }
+      iDestruct (queue_elems_interp_get with "EI") as "PEv"; eauto.
       iSplitL "HNI PEv".
       { iRight. by iFrame. }
       rewrite DOM dom_max_set_fold in RH_WF'.
       destruct RH_WF as (SEQ &  BB). 
       Unshelve. 2: exact None. 
       rewrite bi.sep_assoc.
-      iFrame "ROPA EI'".
+      iFrame "ROPA EI".
       rewrite /rop_interp. iSplit. 
       { iIntros (i_ [=]). }
       iSplitR.
@@ -378,7 +380,6 @@ Section DequeueGhost.
   Qed.
 
   Lemma get_to_free_post
-    PE
   (pbr : loc) (b b1 : nat) ph h fl ndh r i (ndbr1 : Node) (LEb : b ≤ b1)
   pfl (ndfl : Node) (hq : HistQueue) (t br : nat) (rop : option nat) (hist : read_hist)
   (PTR_EQ : pbr = ph)
@@ -408,7 +409,7 @@ Section DequeueGhost.
   hn_interp (pfl, ndfl) -∗
   dangle_auth (Some h) -∗
   (let '(v, nxt) := ndh in ph ↦ v ∗ (ph +ₗ 1) ↦ #nxt) -∗
-  ohv_interp -∗
+  ohv_interp PE -∗
   read_hist_interp hist rop (h + 1) br fl (Some h) -∗
   ((∃ pt : loc, read_head_resources t br pt None ∗ rop_token)
          ∨ read_head_token) -∗
@@ -418,12 +419,13 @@ Section DequeueGhost.
                 queue_inv_inner PE hq0 h0 t0 br0 fl0 rop0 od hist0) ={
            ⊤ ∖ ↑queue_ns,⊤}=∗ emp) -∗
   simple_queue.FreeLater q_sq ↦ #ph -∗
-  queue_elems_interp PE hq (h + 1) -∗
+  queue_elems_interp PE hq -∗
   |={⊤ ∖ ↑queue_ns,⊤}=>
     ∃ (x : Node) (x0 : nat), (let '(v, nxt) := x in pfl ↦ v ∗ (pfl +ₗ 1) ↦ #nxt) ∗
       @me_exact _ q_me_h (h + 1) ∗ @me_exact _ q_me_fl x0 ∗ simple_queue.Head q_sq ↦{
       1 / 2} #ndh.2 ∗ dangle_frag None.
   Proof using.
+    clear PERS_PE. 
     iIntros "#HTH #READ #BR0 #NO_FL #BR1 #BRTH1 #FLTH #PFL_NEQ_D".
     iIntros "CH CFL HEAD' DFRAG HQ AUTHS PQI BR HNI_FL DAUTH HNI OHV RHI RH TOK CLOS FL EI".
 
@@ -530,7 +532,7 @@ Section DequeueGhost.
       by iFrame.
   Qed.
 
-  Lemma check_BR_post PE
+  Lemma check_BR_post
   (h fl : nat) (ph : loc) (ndh : Node) (i r b0 : nat) (hq : HistQueue)
   (t br : nat) (rop : option nat) (hist : read_hist) (pbr : loc) (nbr : Node)
   (READ_BOUND : r ≤ h)
@@ -549,8 +551,8 @@ Section DequeueGhost.
            hn_interp nfl) -∗
   dangle_auth (Some h) -∗
   (let '(v, nxt) := ndh in ph ↦ v ∗ (ph +ₗ 1) ↦ #nxt) -∗
-  PE ndh.1 -∗
-  ohv_interp -∗
+  (* PE ndh.1 -∗ *) (** follows from historical queue *)
+  ohv_interp PE -∗
   read_hist_interp hist rop (h + 1) br fl (Some h) -∗
   ((∃ pt : loc, read_head_resources t br pt None ∗ rop_token)
          ∨ read_head_token) -∗
@@ -560,15 +562,15 @@ Section DequeueGhost.
                 queue_inv_inner PE hq0 h0 t0 br0 fl0 rop0 od hist0) ={
            ⊤ ∖ ↑queue_ns,⊤}=∗ emp) -∗
   BeingRead q_sq ↦ #(pbr, nbr)%core.1 -∗
-  queue_elems_interp PE hq (h + 1) -∗
+  queue_elems_interp PE hq -∗
   |={⊤ ∖ ↑queue_ns,⊤}=>
     dangle_frag (if decide ((pbr, nbr).1 = ph) then Some h else None) ∗
     (⌜(pbr, nbr).1 = ph⌝ ∨ ⌜(pbr, nbr).1 ≠ ph⌝ ∗
      (let '(v, nxt) := ndh in ph ↦ v ∗ (ph +ₗ 1) ↦ #nxt) ∗ PE ndh.1) ∗
     ∃ (b' : nat) (ndbr' : Node), br_lb b' ∗ ⌜b0 ≤ b'⌝ ∗
       ith_node b' ((pbr, nbr).1, ndbr').
-  Proof using.
-    iIntros "#READ #BR0 DFRAG HQ AUTHS PQI FL DAUTH HNI PEv OHV RHI RH TOK CLOS BR EI".
+  Proof using PERS_PE.
+    iIntros "#READ #BR0 DFRAG HQ AUTHS PQI FL DAUTH HNI OHV RHI RH TOK CLOS BR #EI".
     iDestruct (br_lb_bound with "BR0 AUTHS") as %BR0.
     iDestruct (take_snapshot with "[$]") as "#SHT".
     iDestruct (hq_auth_get_ith with "HQ") as "#BRTH'".
@@ -596,6 +598,8 @@ Section DequeueGhost.
       iFrame.      
       iApply fupd_or. iRight. iFrame "HNI".
       rewrite -(bi.sep_True' ⌜ _ ≠ _ ⌝%I). iApply fupd_frame_l. iSplit; [done| ].
+      iDestruct (queue_elems_interp_get _ _ h with "[$]") as "PEv"; eauto. 
+      
       iFrame "PEv". 
       iMod ("CLOS" with "[-]") as "_"; [| done]. 
 
@@ -608,7 +612,7 @@ Section DequeueGhost.
       iDestruct ("ROP" with "[//]") as "(%r_ & %rp & READ_ & RP & ROP)".
       iDestruct (ith_read_hist_compat with "[$] READ_") as %(?&? & READ' & _). 
 
-      iFrame. iFrame "OLDS".
+      iFrame. iFrame "OLDS EI".
       iNext. iFrame (RH_WF ORDER). iSplitR.
       { by iLeft. }
       rewrite /rop_interp.
